theories/Core/Utils.v
@@ -17,6 +17,14 @@ Polymorphic Class MonadBr (M : Type -> Type) : Type :=
 
 Notation rel X Y := (X -> Y -> Prop).
 
+Lemma t_gfp_bt : forall {X} `{CompleteLattice X} (b : mon X),
+  weq (t b (gfp (bt b))) (gfp b).
+Proof.
+  intros. cbn.
+  rewrite <- enhanced_gfp. rewrite t_gfp.
+  reflexivity.
+Qed.
+
 Ltac invert :=
   match goal with
   | h : existT _ _ _ = existT _ _ _ |- _ => dependent induction h
